lemmes sur foldXXX, Array.forallb Array.existsb
git-svn-id: svn+ssh://scm.gforge.inria.fr/svn/coq/branches/native@13563 85f007b7-540e-0410-9357-904b9bb8a0f7

theories/Array/Array.v
@@ -5,6 +5,7 @@ Register array : Type -> Type as array_type.
 Register make : forall {A:Type}, int -> A -> array A as array_make.
 
 Register get : forall {A:Type}, array A -> int -> A as array_get.
+
 Register default : forall {A:Type}, array A -> A as array_default.
 
 Register set : forall {A:Type}, array A -> int -> A -> array A as array_set.
@@ -31,63 +32,89 @@ Axiom get_outofbound : forall A (t:array A) i, (i < length t) = false -> t.[i] =
 
 Axiom get_set_same : forall A t i (a:A), (i < length t) = true -> t.[i<-a].[i] = a.
 Axiom get_set_other : forall A t i j (a:A), i <> j -> t.[i<-a].[j] = t.[j].
+Axiom default_set : forall A t i (a:A), default (t.[i<-a]) = default t.
+
 
 Axiom get_make : forall A (a:A) size i, (make size a).[i] = a.
 Axiom default_make : forall A (a:A) size, (default (make size a)) = a.
 
-(*** TODO: remove this axiom using get_outofbound, get_set_other *)
-Axiom default_set : forall A t i (a:A),
-  default (t.[i<-a]) = default t.
 
 Axiom length_make : forall A size (a:A), 
   length (make size a) = if size <= max_array_length then size else max_array_length.
 Axiom length_set : forall A t i (a:A),
   length (t.[i<-a]) = length t.
 
-Axiom copy_get : forall A (t:array A) i, (copy t).[i] = t.[i].
-Axiom copy_length : forall A (t:array A), length (copy t) = length t.
-(*** TODO: remove this axiom using get_outofbound, copy_get *)
-Axiom copy_default : forall A (t:array A), default (copy t) = default t.
+Axiom get_copy : forall A (t:array A) i, (copy t).[i] = t.[i].
+Axiom length_copy : forall A (t:array A), length (copy t) = length t.
 
-Axiom reroot_get : forall A (t:array A) i, (reroot t).[i] = t.[i].
-Axiom reroot_length : forall A (t:array A), length (copy t) = length t.
-(*** TODO: remove this axiom using get_outofbound, reroot_get *)
-Axiom reroot_default : forall A (t:array A), default (copy t) = default t.
+Axiom get_reroot : forall A (t:array A) i, (reroot t).[i] = t.[i].
+Axiom length_reroot : forall A (t:array A), length (reroot t) = length t.
 
 (* Definition *)
 Definition to_list {A:Type} (t:array A) :=
   let len := length t in
-  if len == 0 then nil
+  if 0 == len then nil
   else foldi_down (fun i l => t.[i] :: l)%list (len - 1) 0 nil.
 
 Definition forallb {A:Type} (f:A->bool) (t:array A) :=
-  forallb (fun i => f (t.[i])) 0 (length t - 1).
+  let len := length t in
+  if 0 == len then true
+  else forallb (fun i => f (t.[i])) 0 (len - 1).
 
 Definition existsb {A:Type} (f:A->bool) (t:array A) :=
-  existsb (fun i => f (t.[i])) 0 (length t - 1).
+  let len := length t in
+  if 0 == len then false
+  else existsb (fun i => f (t.[i])) 0 (len - 1).
 
+(* TODO : We should add init as native and add it *)
 Definition mapi {A B:Type} (f:int->A->B) (t:array A) :=
   let size := length t in
   let def := f size (default t) in
   let tb := make size def in
-  foldi (fun i tb => tb.[i<- f i (t.[i])]) 0 (size - 1) tb.
+  if size == 0 then tb
+  else foldi (fun i tb => tb.[i<- f i (t.[i])]) 0 (size - 1) tb.
 
 Definition map {A B:Type} (f:A->B) :=
   Eval lazy beta delta [mapi] in (mapi (fun i => f)).
 
 Definition foldi_left {A B:Type} (f:int -> A -> B -> A) a (t:array B) :=
-  foldi (fun i a => f i a (t.[i])) 0 (length t - 1) a.
+  let len := length t in
+  if 0 == len then a 
+  else foldi (fun i a => f i a (t.[i])) 0 (len - 1) a.
 
 Definition fold_left {A B:Type} (f: A -> B -> A) a (t:array B) :=
-  foldi (fun i a => f a (t.[i])) 0 (length t - 1) a.
+  let len := length t in
+  if 0 == len then a 
+  else foldi (fun i a => f a (t.[i])) 0 (length t - 1) a.
 
 Definition foldi_right {A B:Type} (f:int -> A -> B -> B) (t:array A) b :=
-  foldi_down (fun i b => f i (t.[i]) b) (length t - 1) 0 b.
+  let len := length t in
+  if 0 == len then b 
+  else foldi_down (fun i b => f i (t.[i]) b) (len - 1) 0 b.
 
 Definition fold_right {A B:Type} (f: A -> B -> B) (t:array A) b :=
-  foldi_down (fun i b => f (t.[i]) b) (length t - 1) 0 b.
+  let len := length t in
+  if 0 == len then b 
+  else foldi_down (fun i b => f (t.[i]) b) (len - 1) 0 b.
 
 (* Lemmas *)
+
+Lemma default_copy : forall A (t:array A), default (copy t) = default t.
+Proof.
+ intros A t;assert (length t < length t = false).
+  apply Bool.not_true_is_false; apply leb_not_gtb; apply leb_refl.
+ rewrite <- (get_outofbound _ (copy t) (length t)), <- (get_outofbound _ t (length t)), get_copy;trivial.
+ rewrite length_copy;trivial.
+Qed.
+
+Lemma reroot_default : forall A (t:array A), default (reroot t) = default t.
+Proof.
+ intros A t;assert (length t < length t = false).
+  apply Bool.not_true_is_false; apply leb_not_gtb; apply leb_refl.
+ rewrite <- (get_outofbound _ (reroot t) (length t)), <- (get_outofbound _ t (length t)), get_reroot;trivial.
+ rewrite length_reroot;trivial.
+Qed.
+
 Lemma get_set_same_default : 
    forall (A : Type) (t : array A) (i : int) ,
        (t .[ i <- default t]) .[ i] = default t.
@@ -105,3 +132,57 @@ Proof.
  case_eq (x < length t);intros Heq;[trivial | ].
  elim Hd;rewrite get_outofbound;trivial.
 Qed.
+
+(* Move *)
+Lemma leb_negb_gtb : forall x y, x <= y = negb (y < x).
+Proof.
+ intros x y;apply Bool.eq_true_iff_eq;split;intros.
+ apply Bool.eq_true_not_negb;apply leb_not_gtb;trivial.
+ rewrite Bool.negb_true_iff, <- Bool.not_true_iff_false in H.
+ rewrite leb_spec; rewrite ltb_spec in H;omega.
+Qed.
+
+Lemma ltb_negb_geb : forall x y, x < y = negb (y <= x).
+Proof.
+ intros;rewrite leb_negb_gtb, Bool.negb_involutive;trivial.
+Qed.
+  
+Lemma fold_left_ind : 
+     forall A B (P : A -> Prop) (f : A -> B -> A) (t:array B),
+     (forall a i, i < length t = true -> P a -> P (f a (t.[i]))) ->
+     forall a, P a ->
+     P (fold_left f a t).
+Proof.
+ intros;unfold fold_left.
+ case_eq (0 == (length t));intros Heq;trivial.
+ apply foldi_ind;trivial.
+ cut (0 < length t = true);[ | 
+  (generalize (leb_0 (length t));rewrite leb_ltb_eqb, Heq, Bool.orb_false_r;trivial)].
+ intros;apply H;trivial.
+ rewrite leb_spec in *;rewrite ltb_spec in *. rewrite to_Z_0 in H1.
+ assert (W:= to_Z_bounded (length t));rewrite sub_spec, to_Z_1, Zmod_small in H3;omega.
+Qed.
+
+Lemma forallb_spec : forall A (f : A -> bool) t,
+  forallb f t = true <-> forall i, i < length t = true -> f (t.[i]) = true.
+Proof.
+ unfold forallb;intros A f t.
+ destruct (reflect_eqb 0 (length t)).
+ split;[intros | trivial].
+ elim (ltb_0 i);rewrite e;trivial.
+ rewrite forallb_spec;split;intros Hi i;intros;apply Hi.
+ apply leb_0. rewrite <- ltb_leb_sub1;auto. rewrite ltb_leb_sub1;auto.
+Qed.
+
+Lemma existsb_spec : forall A (f : A -> bool) t,
+  existsb f t = true <-> exists i, i < length t = true /\ f (t.[i]) = true.
+Proof.
+ unfold existsb;intros A f t.
+ destruct (reflect_eqb 0 (length t)).
+ split;[discriminate | intros [i [Hi _]];rewrite <- e in Hi;elim (ltb_0 _ Hi)].
+ rewrite existsb_spec. repeat setoid_rewrite Bool.andb_true_iff.
+ split;intros [i H];decompose [and] H;clear H;exists i;repeat split;trivial.
+ rewrite ltb_leb_sub1;auto. apply leb_0. rewrite <- ltb_leb_sub1;auto.
+Qed.
+
+
